Port Lia.v

src/lia/Lia.v
@@ -157,44 +157,44 @@ Section certif.
   Section Build_form.
 
     Definition build_not2 i f :=
-      fold (fun f' : BFormula (Formula Z) => N (N f')) 1 i f.
+      fold (fun f' : BFormula (Formula Z) isProp => NOT (NOT f')) 1 i f.
 
-    Variable build_var : vmap -> var -> option (vmap*BFormula (Formula Z)).
+    Variable build_var : vmap -> var -> option (vmap*(BFormula (Formula Z) isProp)).
 
 
-    Definition build_hform vm f : option (vmap*BFormula (Formula Z)) :=
+    Definition build_hform vm f : option (vmap*(BFormula (Formula Z) isProp)) :=
       match f with
         | Form.Fatom h =>
           match build_formula vm h with
-            | Some (vm,f) => Some (vm, A f tt)
+            | Some (vm,f) => Some (vm, A isProp f tt)
             | None => None
           end
-        | Form.Ftrue => Some (vm, TT)
-        | Form.Ffalse => Some (vm, FF)
+        | Form.Ftrue => Some (vm, TT isProp)
+        | Form.Ffalse => Some (vm, FF isProp)
         | Form.Fnot2 i l =>
           match build_var vm (Lit.blit l) with
             | Some (vm, f) =>
               let f' := build_not2 i f in
-              let f'' := if Lit.is_pos l then f' else N f' in
+              let f'' := if Lit.is_pos l then f' else NOT f' in
               Some (vm,f'')
             | None => None
           end
         | Form.Fand args =>
           let n := length args in
-          if n == 0 then Some (vm,TT)
+          if n == 0 then Some (vm,TT isProp)
           else
-            foldi (fun i f1 => match f1 with | Some(vm',f1') => let l := (args.[i]) in match build_var vm' (Lit.blit l) with | Some(vm2,f2) => let f2' := if Lit.is_pos l then f2 else N f2 in Some(vm2,Cj f1' f2') | None => None end | None => None end) 1 (n-1) (let l := args.[0] in
+            foldi (fun i f1 => match f1 with | Some(vm',f1') => let l := (args.[i]) in match build_var vm' (Lit.blit l) with | Some(vm2,f2) => let f2' := if Lit.is_pos l then f2 else NOT f2 in Some(vm2,AND f1' f2') | None => None end | None => None end) 1 (n-1) (let l := args.[0] in
               match build_var vm (Lit.blit l) with
-                | Some (vm',f) => if Lit.is_pos l then Some (vm',f) else Some (vm',N f)
+                | Some (vm',f) => if Lit.is_pos l then Some (vm',f) else Some (vm',NOT f)
                 | None => None
               end)
         | Form.For args =>
           let n := length args in
-          if n == 0 then Some (vm,FF)
+          if n == 0 then Some (vm,FF isProp)
           else
-            foldi (fun i f1 => match f1 with | Some(vm',f1') => let l := (args.[i]) in match build_var vm' (Lit.blit l) with | Some(vm2,f2) => let f2' := if Lit.is_pos l then f2 else N f2 in Some(vm2,D f1' f2') | None => None end | None => None end) 1 (n-1) (let l := args.[0] in
+            foldi (fun i f1 => match f1 with | Some(vm',f1') => let l := (args.[i]) in match build_var vm' (Lit.blit l) with | Some(vm2,f2) => let f2' := if Lit.is_pos l then f2 else NOT f2 in Some(vm2,OR f1' f2') | None => None end | None => None end) 1 (n-1) (let l := args.[0] in
               match build_var vm (Lit.blit l) with
-                | Some (vm',f) => if Lit.is_pos l then Some (vm',f) else Some (vm',N f)
+                | Some (vm',f) => if Lit.is_pos l then Some (vm',f) else Some (vm',NOT f)
                 | None => None
               end)
         | Form.Fxor a b =>
@@ -202,26 +202,26 @@ Section certif.
             | Some (vm1, f1) =>
               match build_var vm1 (Lit.blit b) with
                 | Some (vm2, f2) =>
-                  let f1' := if Lit.is_pos a then f1 else N f1 in
-                  let f2' := if Lit.is_pos b then f2 else N f2 in
-                  Some (vm2, Cj (D f1' f2') (D (N f1') (N f2')))
+                  let f1' := if Lit.is_pos a then f1 else NOT f1 in
+                  let f2' := if Lit.is_pos b then f2 else NOT f2 in
+                  Some (vm2, AND (OR f1' f2') (OR (NOT f1') (NOT f2')))
                 | None => None
               end
             | None => None
           end
         | Form.Fimp args =>
           let n := length args in
-          if n == 0 then Some (vm,TT)
+          if n == 0 then Some (vm,TT isProp)
           else if n <= 1 then
             let l := args.[0] in
             match build_var vm (Lit.blit l) with
-              | Some (vm',f) => if Lit.is_pos l then Some (vm',f) else Some (vm',N f)
+              | Some (vm',f) => if Lit.is_pos l then Some (vm',f) else Some (vm',NOT f)
               | None => None
             end
           else
-            foldi_down (fun i f1 => match f1 with | Some(vm',f1') => let l := (args.[i]) in match build_var vm' (Lit.blit l) with | Some(vm2,f2) => let f2' := if Lit.is_pos l then f2 else N f2 in Some(vm2,I f2' None f1') | None => None end | None => None end) (n-2) 0 (let l := args.[n-1] in
+            foldi_down (fun i f1 => match f1 with | Some(vm',f1') => let l := (args.[i]) in match build_var vm' (Lit.blit l) with | Some(vm2,f2) => let f2' := if Lit.is_pos l then f2 else NOT f2 in Some(vm2,IMPL f2' None f1') | None => None end | None => None end) (n-2) 0 (let l := args.[n-1] in
               match build_var vm (Lit.blit l) with
-                | Some (vm',f) => if Lit.is_pos l then Some (vm',f) else Some (vm',N f)
+                | Some (vm',f) => if Lit.is_pos l then Some (vm',f) else Some (vm',NOT f)
                 | None => None
               end)
         | Form.Fiff a b =>
@@ -229,9 +229,9 @@ Section certif.
             | Some (vm1, f1) =>
               match build_var vm1 (Lit.blit b) with
                 | Some (vm2, f2) =>
-                  let f1' := if Lit.is_pos a then f1 else N f1 in
-                  let f2' := if Lit.is_pos b then f2 else N f2 in
-                  Some (vm2, Cj (D f1' (N f2')) (D (N f1') f2'))
+                  let f1' := if Lit.is_pos a then f1 else NOT f1 in
+                  let f2' := if Lit.is_pos b then f2 else NOT f2 in
+                  Some (vm2, AND (OR f1' (NOT f2')) (OR (NOT f1') f2'))
                 | None => None
               end
             | None => None
@@ -243,10 +243,10 @@ Section certif.
                 | Some (vm2, f2) =>
                   match build_var vm2 (Lit.blit c) with
                     | Some (vm3, f3) =>
-                      let f1' := if Lit.is_pos a then f1 else N f1 in
-                      let f2' := if Lit.is_pos b then f2 else N f2 in
-                      let f3' := if Lit.is_pos c then f3 else N f3 in
-                      Some (vm3, D (Cj f1' f2') (Cj (N f1') f3'))
+                      let f1' := if Lit.is_pos a then f1 else NOT f1 in
+                      let f2' := if Lit.is_pos b then f2 else NOT f2 in
+                      let f3' := if Lit.is_pos c then f3 else NOT f3 in
+                      Some (vm3, OR (AND f1' f2') (AND (NOT f1') f3'))
                     | None => None
                   end
                 | None => None
@@ -271,14 +271,14 @@ Section certif.
     let l := Lit.neg l in
     match build_form vm (get_form (Lit.blit l)) with
       | Some (vm,f) =>
-        let f := if Lit.is_pos l then f else N f in
+        let f := if Lit.is_pos l then f else NOT f in
         Some (vm,f)
       | None => None
     end.
 
 
   Fixpoint build_clause_aux vm (cl:list _lit) {struct cl} :
-    option (vmap * BFormula (Formula Z)) :=
+    option (vmap * BFormula (Formula Z) isProp) :=
     match cl with
     | nil => None
     | l::nil => build_nlit vm l
@@ -286,7 +286,7 @@ Section certif.
       match build_nlit vm l with
       | Some (vm,bf1) =>
         match build_clause_aux vm cl with
-        | Some (vm,bf2) => Some (vm, Cj bf1 bf2)
+        | Some (vm,bf2) => Some (vm, AND bf1 bf2)
         | _ => None
         end
       | None => None
@@ -295,7 +295,7 @@ Section certif.
 
   Definition build_clause vm cl :=
     match build_clause_aux vm cl with
-    | Some (vm, bf) => Some (vm, I bf None FF)
+    | Some (vm, bf) => Some (vm, IMPL bf None (FF isProp))
     | None => None
     end.
 
@@ -477,14 +477,16 @@ Section certif.
     Definition bounded_formula (p:positive) (f:Formula Z) :=
       bounded_pexpr p (f.(Flhs)) &&  bounded_pexpr p (f.(Frhs)).
 
-    Fixpoint bounded_bformula (p:positive) (bf:BFormula (Formula Z)) :=
+    Fixpoint bounded_bformula (p:positive) {k:kind} (bf:BFormula (Formula Z) k) : bool :=
       match bf with
-      | @TT _ | @FF _ | @X _ _ _ _ _ => true
-      | A f _ => bounded_formula p f
-      | Cj bf1 bf2
-      | D bf1 bf2
-      | I bf1 _ bf2 => bounded_bformula p bf1 && bounded_bformula p bf2
-      | N bf => bounded_bformula p bf
+      | @TT _ _ _ _ _ | @FF _ _ _ _ _ | @X _ _ _ _ _ _ => true
+      | A _ f _ => bounded_formula p f
+      | AND bf1 bf2
+      | OR bf1 bf2
+      | IMPL bf1 _ bf2 => bounded_bformula p bf1 && bounded_bformula p bf2
+      | NOT bf => bounded_bformula p bf
+      | IFF bf1 bf2 => bounded_bformula p bf1 && bounded_bformula p bf2
+      | EQ bf1 bf2 => bounded_bformula p bf1 && bounded_bformula p bf2
       end.
 
     Definition interp_vmap (vm:vmap) p :=
@@ -958,7 +960,7 @@ Transparent build_z_atom.
            nth_error (snd vm) (nat_of_P (fst vm - p) - 1) =
            nth_error (snd vm')(nat_of_P (fst vm' - p) - 1)) /\
           bounded_formula (fst vm') f /\
-          (interp_bool t_i (interp_atom a) <->Zeval_formula (interp_vmap vm') f).
+          (interp_bool t_i (interp_atom a) <->Zeval_formula (interp_vmap vm') isProp f).
     Proof.
       intros a vm vm' f t.
       destruct a;simpl;try discriminate.
@@ -1011,7 +1013,7 @@ Transparent build_z_atom.
            nth_error (snd vm) (nat_of_P (fst vm - p) - 1) =
            nth_error (snd vm')(nat_of_P (fst vm' - p) - 1)) /\
           bounded_formula (fst vm') f /\
-          (interp_form_hatom h' <-> Zeval_formula (interp_vmap vm') f).
+          (interp_form_hatom h' <-> Zeval_formula (interp_vmap vm') isProp f).
     Proof.
       unfold build_formula;intros h.
       unfold Atom.interp_form_hatom, Atom.interp_hatom.
@@ -1026,14 +1028,14 @@ Transparent build_z_atom.
     Qed.
 
 
-    Local Notation eval_f := (eval_f (fun x => x)).
+    Local Notation eval_f := (eval_f (fun k x => x)).
 
-    Lemma build_not2_pos_correct : forall vm f l i,
+    Lemma build_not2_pos_correct : forall vm (f:GFormula isProp) l i,
       bounded_bformula (fst vm) f -> (rho (Lit.blit l) <-> eval_f (Zeval_formula (interp_vmap vm)) f) -> Lit.is_pos l -> bounded_bformula (fst vm) (build_not2 i f) /\ (Form.interp interp_form_hatom interp_form_hatom_bv t_form (Form.Fnot2 i l) <-> eval_f (Zeval_formula (interp_vmap vm)) (build_not2 i f)).
     Proof.
       simpl; intros vm f l i H1 H2 H3; split; unfold build_not2.
       apply fold_ind; auto.
-      apply (fold_ind2 _ _ (fun b f' => b = true <-> eval_f (Zeval_formula (interp_vmap vm)) f')).
+      apply (fold_ind2 _ _ (fun b (f':GFormula isProp) => b = true <-> eval_f (Zeval_formula (interp_vmap vm)) f')).
       unfold Lit.interp; rewrite H3; auto.
       intros b f' H4; rewrite negb_involutive; simpl; split.
       intros Hb H5; apply H5; rewrite <- H4; auto.
@@ -1041,12 +1043,12 @@ Transparent build_z_atom.
     Qed.
 
 
-    Lemma build_not2_neg_correct : forall vm f l i,
-      bounded_bformula (fst vm) f -> (rho (Lit.blit l) <-> eval_f (Zeval_formula (interp_vmap vm)) f) -> Lit.is_pos l = false -> bounded_bformula (fst vm) (N (build_not2 i f)) /\ (Form.interp interp_form_hatom interp_form_hatom_bv t_form (Form.Fnot2 i l) <-> eval_f (Zeval_formula (interp_vmap vm)) (N (build_not2 i f))).
+    Lemma build_not2_neg_correct : forall vm (f:GFormula isProp) l i,
+      bounded_bformula (fst vm) f -> (rho (Lit.blit l) <-> eval_f (Zeval_formula (interp_vmap vm)) f) -> Lit.is_pos l = false -> bounded_bformula (fst vm) (NOT (build_not2 i f)) /\ (Form.interp interp_form_hatom interp_form_hatom_bv t_form (Form.Fnot2 i l) <-> eval_f (Zeval_formula (interp_vmap vm)) (NOT (build_not2 i f))).
     Proof.
       simpl; intros vm f l i H1 H2 H3; split; unfold build_not2.
       apply fold_ind; auto.
-      apply (fold_ind2 _ _ (fun b f' => b = true <-> ~ eval_f (Zeval_formula (interp_vmap vm)) f')).
+      apply (fold_ind2 _ _ (fun b (f':GFormula isProp) => b = true <-> ~ eval_f (Zeval_formula (interp_vmap vm)) f')).
       unfold Lit.interp; rewrite H3; unfold Var.interp; split.
       intros H4 H5; rewrite <- H2 in H5; rewrite H5 in H4; discriminate.
       intro H4; case_eq (rho (Lit.blit l)); auto; intro H5; elim H4; rewrite <- H2; auto.
@@ -1059,42 +1061,73 @@ Transparent build_z_atom.
     Lemma bounded_bformula_le :
      forall p p',
        (nat_of_P p <= nat_of_P p')%nat ->
-        forall bf,
+        forall (bf:BFormula (Formula Z) isProp),
         bounded_bformula p bf -> bounded_bformula p' bf.
     Proof.
       unfold is_true;induction bf;simpl;trivial.
-      destruct a;unfold bounded_formula;simpl.
-      rewrite andb_true_iff;intros (H1, H2).
-      rewrite (bounded_pexpr_le _ _ H _ H1), (bounded_pexpr_le _ _ H _ H2);trivial.
-      rewrite !andb_true_iff;intros (H1, H2);auto.
-      rewrite !andb_true_iff;intros (H1, H2);auto.
-      rewrite !andb_true_iff;intros (H1, H2);auto.
+      - destruct a;unfold bounded_formula;simpl.
+        rewrite andb_true_iff;intros (H1, H2).
+        rewrite (bounded_pexpr_le _ _ H _ H1), (bounded_pexpr_le _ _ H _ H2);trivial.
+      - rewrite !andb_true_iff;intros (H1, H2);auto.
+      - rewrite !andb_true_iff;intros (H1, H2);auto.
+      - rewrite !andb_true_iff;intros (H1, H2);auto.
+      - rewrite !andb_true_iff;intros (H1, H2);auto.
+      - rewrite !andb_true_iff;intros (H1, H2);auto.
     Qed.
 
-    Lemma interp_bformula_le :
-     forall vm vm',
-       (forall (p : positive),
-         (nat_of_P p < nat_of_P (fst vm))%nat ->
-         nth_error (snd vm) (nat_of_P (fst vm - p) - 1) =
-         nth_error (snd vm') (nat_of_P (fst vm' - p) - 1)) ->
-     forall bf,
-       bounded_bformula (fst vm) bf ->
-       (eval_f (Zeval_formula (interp_vmap vm)) bf <->
-       eval_f (Zeval_formula (interp_vmap vm')) bf).
-    Proof.
-      intros vm vm' Hnth.
-      unfold is_true;induction bf;simpl;try tauto.
-      destruct t;unfold bounded_formula;simpl.
-      rewrite andb_true_iff;intros (H1, H2).
-      rewrite !(interp_pexpr_le _ _ Hnth);tauto.
-      rewrite andb_true_iff;intros (H1,H2);rewrite IHbf1, IHbf2;tauto.
-      rewrite andb_true_iff;intros (H1,H2);rewrite IHbf1, IHbf2;tauto.
-      rewrite andb_true_iff;intros (H1,H2);rewrite IHbf1, IHbf2;tauto.
-    Qed.
+    Section Interp_bformula.
+
+      Variables vm vm' : positive * list atom.
+      Variable Hnth : forall p : positive,
+          (Pos.to_nat p < Pos.to_nat (fst vm))%nat ->
+          nth_error (snd vm) (Pos.to_nat (fst vm - p) - 1) =
+          nth_error (snd vm') (Pos.to_nat (fst vm' - p) - 1).
+
+      Definition P k : GFormula k -> Prop :=
+        match k as k return GFormula k -> Prop with
+        | isProp => fun (bf:BFormula (Formula Z) isProp) =>
+                      bounded_bformula (fst vm) bf ->
+                      (eval_f (Zeval_formula (interp_vmap vm)) bf <->
+                       eval_f (Zeval_formula (interp_vmap vm')) bf)
+        | isBool => fun (bf:BFormula (Formula Z) isBool) =>
+                      bounded_bformula (fst vm) bf ->
+                      (eval_f (Zeval_formula (interp_vmap vm)) bf =
+                       eval_f (Zeval_formula (interp_vmap vm')) bf)
+        end.
+
+      Lemma interp_bformula_le_gen : forall k f, P k f.
+      Proof.
+        intro k. induction f as [k|k|k t|k t a|k f1 IHf1 f2 IHf2|k f1 IHf1 f2 IHf2|k f1 IHf1|k f1 IHf1 o f2 IHf2|k f1 IHf1 f2 IHf2|f1 IHf1 f2 IHf2]; unfold P in *;
+                   try (destruct k; simpl; tauto);
+                   try (destruct k; simpl; unfold is_true;rewrite andb_true_iff;intros (H1,H2);rewrite IHf1, IHf2;tauto).
+        - destruct k; simpl;
+            destruct t;unfold bounded_formula;simpl;
+              unfold is_true;rewrite andb_true_iff;intros (H1, H2);
+                rewrite !(interp_pexpr_le _ _ Hnth);tauto.
+        - destruct k; simpl; intro H; now rewrite IHf1.
+        - destruct k; simpl.
+          + unfold is_true;rewrite andb_true_iff;intros (H1, H2).
+            split.
+            * intros H3 H4. rewrite <- IHf2; auto. apply H3. now rewrite IHf1.
+            * intros H3 H4. rewrite IHf2; auto. apply H3. now rewrite <- IHf1.
+          + unfold is_true;rewrite andb_true_iff;intros (H1, H2).
+            now rewrite IHf1, IHf2.
+        - simpl. unfold is_true;rewrite andb_true_iff;intros (H1, H2).
+          now rewrite IHf1, IHf2.
+      Qed.
+
+      Lemma interp_bformula_le :
+        forall (bf:BFormula (Formula Z) isProp),
+          bounded_bformula (fst vm) bf ->
+          (eval_f (Zeval_formula (interp_vmap vm)) bf <->
+           eval_f (Zeval_formula (interp_vmap vm')) bf).
+      Proof. exact (interp_bformula_le_gen isProp). Qed.
+
+    End Interp_bformula.
 
 
     Lemma build_hform_correct :
-      forall (build_var : vmap -> var -> option (vmap*BFormula (Formula Z))),
+      forall (build_var : vmap -> var -> option (vmap*BFormula (Formula Z) isProp)),
         (forall v vm vm' bf,
           build_var vm v = Some (vm', bf) ->
           wf_vmap vm ->
@@ -1130,7 +1163,7 @@ Transparent build_z_atom.
       (* Fand *)
       simpl; unfold afold_left; case (length l == 0).
       intro H; inversion H; subst vm'; subst bf; simpl; intro H1; split; auto with smtcoq_core; split; [lia| ]; do 3 (split; auto with smtcoq_core).
-      revert vm' bf; apply (foldi_ind2 _ _ (fun f1 b => forall vm' bf, f1 = Some (vm', bf) -> wf_vmap vm -> wf_vmap vm' /\ (Pos.to_nat (fst vm) <= Pos.to_nat (fst vm'))%nat /\ (forall p : positive, (Pos.to_nat p < Pos.to_nat (fst vm))%nat -> nth_error (snd vm) (Pos.to_nat (fst vm - p) - 1) = nth_error (snd vm') (Pos.to_nat (fst vm' - p) - 1)) /\ bounded_bformula (fst vm') bf /\ (b = true <-> eval_f (Zeval_formula (interp_vmap vm')) bf))).
+      revert vm' bf; apply (foldi_ind2 _ _ (fun f1 b => forall vm' (bf:BFormula (Formula Z) isProp), f1 = Some (vm', bf) -> wf_vmap vm -> wf_vmap vm' /\ (Pos.to_nat (fst vm) <= Pos.to_nat (fst vm'))%nat /\ (forall p : positive, (Pos.to_nat p < Pos.to_nat (fst vm))%nat -> nth_error (snd vm) (Pos.to_nat (fst vm - p) - 1) = nth_error (snd vm') (Pos.to_nat (fst vm' - p) - 1)) /\ bounded_bformula (fst vm') bf /\ (b = true <-> eval_f (Zeval_formula (interp_vmap vm')) bf))).
       intros vm' bf; case_eq (build_var vm (Lit.blit (l .[ 0]))); try discriminate; intros [vm0 f] Heq; case_eq (Lit.is_pos (l .[ 0])); intros Heq2 H1 H2; inversion H1; subst vm'; subst bf; destruct (Hbv _ _ _ _ Heq H2) as [H10 [H11 [H12 [H13 H14]]]]; do 4 (split; auto); unfold Lit.interp; rewrite Heq2; auto; simpl; split.
       intros H3 H4; rewrite <- H14 in H4; rewrite H4 in H3; discriminate.
       intro H3; case_eq (Var.interp rho (Lit.blit (l .[ 0]))); auto; intro H4; elim H3; rewrite <- H14; auto.
@@ -1142,7 +1175,7 @@ Transparent build_z_atom.
       (* For *)
       simpl; unfold afold_left; case (length l == 0).
       intro H; inversion H; subst vm'; subst bf; simpl; intro H1; split; auto with smtcoq_core; split; [lia| ]; do 3 (split; auto with smtcoq_core); discriminate.
-      revert vm' bf; apply (foldi_ind2 _ _ (fun f1 b => forall vm' bf, f1 = Some (vm', bf) -> wf_vmap vm -> wf_vmap vm' /\ (Pos.to_nat (fst vm) <= Pos.to_nat (fst vm'))%nat /\ (forall p : positive, (Pos.to_nat p < Pos.to_nat (fst vm))%nat -> nth_error (snd vm) (Pos.to_nat (fst vm - p) - 1) = nth_error (snd vm') (Pos.to_nat (fst vm' - p) - 1)) /\ bounded_bformula (fst vm') bf /\ (b = true <-> eval_f (Zeval_formula (interp_vmap vm')) bf))).
+      revert vm' bf; apply (foldi_ind2 _ _ (fun f1 b => forall vm' (bf:BFormula (Formula Z) isProp), f1 = Some (vm', bf) -> wf_vmap vm -> wf_vmap vm' /\ (Pos.to_nat (fst vm) <= Pos.to_nat (fst vm'))%nat /\ (forall p : positive, (Pos.to_nat p < Pos.to_nat (fst vm))%nat -> nth_error (snd vm) (Pos.to_nat (fst vm - p) - 1) = nth_error (snd vm') (Pos.to_nat (fst vm' - p) - 1)) /\ bounded_bformula (fst vm') bf /\ (b = true <-> eval_f (Zeval_formula (interp_vmap vm')) bf))).
       intros vm' bf; case_eq (build_var vm (Lit.blit (l .[ 0]))); try discriminate; intros [vm0 f] Heq; case_eq (Lit.is_pos (l .[ 0])); intros Heq2 H1 H2; inversion H1; subst vm'; subst bf; destruct (Hbv _ _ _ _ Heq H2) as [H10 [H11 [H12 [H13 H14]]]]; do 4 (split; auto with smtcoq_core); unfold Lit.interp; rewrite Heq2; auto with smtcoq_core; simpl; split.
       intros H3 H4; rewrite <- H14 in H4; rewrite H4 in H3; discriminate.
       intro H3; case_eq (Var.interp rho (Lit.blit (l .[ 0]))); auto with smtcoq_core; intro H4; elim H3; rewrite <- H14; auto with smtcoq_core.
@@ -1152,13 +1185,14 @@ Transparent build_z_atom.
       simpl; rewrite (bounded_bformula_le _ _ H11 _ H8); case (Lit.is_pos (l .[ i])); rewrite H13; auto with smtcoq_core.
       simpl; rewrite (interp_bformula_le _ _ H12 _ H8) in H9; rewrite <- H9; case_eq (Lit.is_pos (l .[ i])); intro Heq2; simpl; rewrite <- H14; unfold Lit.interp; rewrite Heq2; split; case (Var.interp rho (Lit.blit (l .[ i]))); try rewrite orb_false_r; try rewrite orb_true_r; auto with smtcoq_core; try (intros [H20|H20]; auto with smtcoq_core; discriminate); right; intro H20; discriminate.
       (* Fimp *)
+      {
       simpl; unfold afold_right; case (length l == 0).
       intro H; inversion H; subst vm'; subst bf; simpl; intro H1; split; auto with smtcoq_core; split; [lia| ]; do 3 (split; auto with smtcoq_core).
       case (length l <= 1).
       case_eq (build_var vm (Lit.blit (l .[ 0]))); try discriminate; intros [vm0 f] Heq; case_eq (Lit.is_pos (l .[ 0])); intros Heq2 H1 H2; inversion H1; subst vm'; subst bf; destruct (Hbv _ _ _ _ Heq H2) as [H3 [H4 [H5 [H6 H7]]]]; do 4 (split; auto with smtcoq_core); unfold Lit.interp; rewrite Heq2; auto with smtcoq_core; simpl; split.
       intros H8 H9; rewrite <- H7 in H9; rewrite H9 in H8; discriminate.
       intro H8; case_eq (Var.interp rho (Lit.blit (l .[ 0]))); auto with smtcoq_core; intro H9; rewrite H7 in H9; elim H8; auto with smtcoq_core.
-      revert vm' bf; apply (foldi_down_ind2 _ _ (fun f1 b => forall vm' bf, f1 = Some (vm', bf) -> wf_vmap vm -> wf_vmap vm' /\ (Pos.to_nat (fst vm) <= Pos.to_nat (fst vm'))%nat /\ (forall p : positive, (Pos.to_nat p < Pos.to_nat (fst vm))%nat -> nth_error (snd vm) (Pos.to_nat (fst vm - p) - 1) = nth_error (snd vm') (Pos.to_nat (fst vm' - p) - 1)) /\ bounded_bformula (fst vm') bf /\ (b = true <-> eval_f (Zeval_formula (interp_vmap vm')) bf))).
+      revert vm' bf; apply (foldi_down_ind2 _ _ (fun f1 b => forall vm' (bf:BFormula (Formula Z) isProp), f1 = Some (vm', bf) -> wf_vmap vm -> wf_vmap vm' /\ (Pos.to_nat (fst vm) <= Pos.to_nat (fst vm'))%nat /\ (forall p : positive, (Pos.to_nat p < Pos.to_nat (fst vm))%nat -> nth_error (snd vm) (Pos.to_nat (fst vm - p) - 1) = nth_error (snd vm') (Pos.to_nat (fst vm' - p) - 1)) /\ bounded_bformula (fst vm') bf /\ (b = true <-> eval_f (Zeval_formula (interp_vmap vm')) bf))).
       intros vm' bf; case_eq (build_var vm (Lit.blit (l .[ length l - 1]))); try discriminate; intros [vm0 f] Heq; case_eq (Lit.is_pos (l .[ length l - 1])); intros Heq2 H1 H2; inversion H1; subst vm'; subst bf; destruct (Hbv _ _ _ _ Heq H2) as [H10 [H11 [H12 [H13 H14]]]]; do 4 (split; auto with smtcoq_core); unfold Lit.interp; rewrite Heq2; auto with smtcoq_core; simpl; split.
       intros H3 H4; rewrite <- H14 in H4; rewrite H4 in H3; discriminate.
       intro H3; case_eq (Var.interp rho (Lit.blit (l .[ length l - 1]))); auto with smtcoq_core; intro H4; elim H3; rewrite <- H14; auto with smtcoq_core.
@@ -1166,7 +1200,21 @@ Transparent build_z_atom.
       intros p H15; rewrite H7; auto with smtcoq_core; apply H12; eauto with smtcoq_core arith.
       split.
       simpl; rewrite (bounded_bformula_le _ _ H11 _ H8); case (Lit.is_pos (l .[ i])); rewrite H13; auto with smtcoq_core.
-      simpl; rewrite (interp_bformula_le _ _ H12 _ H8) in H9; rewrite <- H9; case_eq (Lit.is_pos (l .[ i])); intro Heq2; simpl; rewrite <- H14; unfold Lit.interp; rewrite Heq2; split; case (Var.interp rho (Lit.blit (l .[ i]))); auto with smtcoq_core; try discriminate; simpl; intro H; apply H; discriminate.
+      simpl; rewrite (interp_bformula_le _ _ H12 _ H8) in H9.
+      case_eq (Lit.is_pos (l .[ i])); intro Heq2; simpl.
+      - unfold Lit.interp. rewrite Heq2. split.
+        + revert H14. case (Var.interp rho (Lit.blit (l .[ i]))); simpl.
+          * intros H101 H102 H103. now rewrite <- H9.
+          * intros H101 H102 H103. rewrite <- H101 in H103. discriminate.
+        + revert H14. case (Var.interp rho (Lit.blit (l .[ i]))); simpl; auto.
+          intros H101 H102. rewrite H9. apply H102. now rewrite <- H101.
+      - unfold Lit.interp. rewrite Heq2. split.
+        + revert H14. case (Var.interp rho (Lit.blit (l .[ i]))); simpl.
+          * intros H101 H102 H103. elim H103. now rewrite <- H101.
+          * intros H101 H102 H103. now rewrite <- H9.
+        + revert H14. case (Var.interp rho (Lit.blit (l .[ i]))); simpl; auto.
+          intros H101 H102. rewrite H9. apply H102. now rewrite <- H101.
+      }
       (* Fxor *)
       simpl; case_eq (build_var vm (Lit.blit a)); try discriminate; intros [vm1 f1] Heq1; case_eq (build_var vm1 (Lit.blit b)); try discriminate; intros [vm2 f2] Heq2 H1 H2; inversion H1; subst vm'; subst bf; destruct (Hbv _ _ _ _ Heq1 H2) as [H3 [H4 [H5 [H6 H7]]]]; destruct (Hbv _ _ _ _ Heq2 H3) as [H8 [H9 [H10 [H11 H12]]]]; split; auto with smtcoq_core; split; [eauto with smtcoq_core arith| ]; split.
       intros p H18; rewrite H5; auto with smtcoq_core; rewrite H10; eauto with smtcoq_core arith.
@@ -1293,7 +1341,7 @@ Transparent build_z_atom.
         ( match build_nlit vm a with
           | Some (vm0, bf1) =>
           match build_clause_aux vm0 (i::l) with
-          | Some (vm1, bf2) => Some (vm1, Cj bf1 bf2)
+          | Some (vm1, bf2) => Some (vm1, AND bf1 bf2)
           | None => None
           end
          | None => None
